tools/gen_lemmas.ml
@@ -324,12 +324,11 @@ let traces_enabled_lemma mem isa id =
     | Some regs when not mem -> List.map (fun r -> r ^ " \\<in> invoked_regs") regs
     | _ -> []
   in
-  let invokes_mem_caps_assm =
-    if IdSet.mem id isa.invokes_mem_caps then ["invokes_mem_caps"] else
-    if not (IdSet.disjoint f.trans_calls isa.cap_load_funs) then ["\\<not>invokes_mem_caps"] else
-    []
+  let invoked_indirect_assms = match Bindings.find_opt id isa.invoked_indirect_regs with
+    | Some regs -> List.map (fun r -> r ^ " \\<in> invoked_indirect_regs") regs
+    | None -> if IdSet.disjoint f.trans_calls isa.cap_load_funs then [] else ["\\<not>invokes_indirect_caps"]
   in
-  let assms = cap_assm @ arg_assms @ eq_assms @ ret_typ_assm @ invoked_reg_assms @ invokes_mem_caps_assm in
+  let assms = cap_assm @ arg_assms @ eq_assms @ ret_typ_assm @ invoked_reg_assms @ invoked_indirect_assms in
   let using = if assms = [] then "" else " assms: assms" in
   { name = "traces_enabled_" ^ name; attrs = "[traces_enabledI]";
     assms; unfolding = [(name ^ "_def"); "bind_assoc"]; using = [];
